refactor: completely strip away game details from syntax/semantics definitions

KripkeGameAnalysis/Basic.lean
@@ -8,6 +8,94 @@ import Mathlib.Data.Fintype.Card
 
 import KripkeGameAnalysis.GenericExtras.FinsetEquivCharacteristic
 
+inductive ModalFormula (vars : Type) : Type where
+| var : vars → ModalFormula vars
+| neg : ModalFormula vars → ModalFormula vars
+| and : ModalFormula vars → ModalFormula vars → ModalFormula vars
+| box : ModalFormula vars → ModalFormula vars
+
+namespace ModalFormula
+  variable {vars : Type}
+
+  abbrev not := fun (φ: ModalFormula vars) => neg φ
+  abbrev or := fun (φ1 φ2: ModalFormula vars) => not (and (not φ1) (not φ2))
+  abbrev implies := fun (φ1 φ2: ModalFormula vars) => or (not φ1) φ2
+  abbrev dia := fun (φ: ModalFormula vars) => not (box (not φ))
+end ModalFormula
+
+def KripkeFrame (vertices : Type) : Type := vertices → vertices → Bool
+namespace KripkeFrame
+  def vertices (_ : KripkeFrame v) : Type := v
+  def accessible (frame : KripkeFrame v) (i j : frame.vertices) : Bool := frame i j
+
+  def Valuation (frame : KripkeFrame v) (vars : Type) : Type := vars → frame.vertices → Bool
+
+  def Valuation.decideSatisfaction {frame : KripkeFrame v} [Fintype frame.vertices]
+                                   (i : frame.vertices) (fml : ModalFormula vars) (val : frame.Valuation vars) : Bool :=
+  match fml with
+    | ModalFormula.var x => val x i
+    | ModalFormula.neg φ => !(val.decideSatisfaction i φ)
+    | ModalFormula.and φ1 φ2 => val.decideSatisfaction i φ1 && val.decideSatisfaction i φ2
+    | ModalFormula.box φ => decide (∀j: frame.vertices, if frame.accessible i j then val.decideSatisfaction j φ else true)
+
+end KripkeFrame
+
+/-- A Kripke frame of `frameSize` possible worlds is a directed graph with `frameSize` vertices.
+
+We think of the vertices in the graph as being numbered from `0` to `frameSize - 1`, inclusive,
+and we think the `j`-th vertex is accessible from the `i`-th vertex if and only if there is an edge from `i` to `j`.
+
+The graph, then, is represented by a function that takes two natural numbers `n` and `m` as input,
+and returns `true` if there is an edge from vertex `n` to vertex `m`, and `false` otherwise.
+-/
+def FiniteKripkeFrame (frameSize : Nat) : Type := KripkeFrame (Fin frameSize)
+namespace FiniteKripkeFrame
+  instance (frame : FiniteKripkeFrame n) : Fintype frame.vertices := inferInstanceAs (Fintype (Fin n))
+  instance (frame : FiniteKripkeFrame n) : DecidableEq frame.vertices := inferInstanceAs (DecidableEq (Fin n))
+
+  def allNodes (frame : FiniteKripkeFrame n) : Finset frame.vertices := Finset.univ
+  lemma allNodes_card_eq_frameSize (frame : FiniteKripkeFrame n) : frame.allNodes.card = n :=
+    by apply Fintype.card_fin
+
+  def accessibilityRelationCount (frame : FiniteKripkeFrame n) : ℕ :=
+    ((frame.allNodes.product (frame.allNodes)).filter (fun a => frame.accessible a.fst a.snd)).card
+
+  structure FiniteValuation (frame : FiniteKripkeFrame n) (vars : Type) [Fintype vars] [DecidableEq vars] where
+    valuation : frame.Valuation vars
+
+  namespace FiniteValuation
+    def equivToFinSetRepresentation {finVars : Type} {frame : FiniteKripkeFrame n} [Fintype finVars] [DecidableEq finVars]:
+                                    (frame.FiniteValuation finVars) ≃ (Finset (finVars × frame.vertices)) :=
+      let valPowersetEquiv : (frame.Valuation finVars) ≃ (Finset (finVars × frame.vertices)) := finsetProdEquivCurriedCharacteristic.symm
+      let valEquiv : (frame.FiniteValuation finVars) ≃ (frame.Valuation finVars) := {
+        toFun := fun val => val.valuation,
+        invFun := fun val => { valuation := val },
+        left_inv := by intro val; simp,
+        right_inv := by intro val; simp
+      }
+      valEquiv.trans valPowersetEquiv
+  end FiniteValuation
+
+  def allValuations (frame : FiniteKripkeFrame n) (finVars : Type) [varsFin : Fintype finVars] [DecidableEq finVars] : Finset (frame.FiniteValuation finVars) :=
+    let valuationsAsPsets := (Finset.product varsFin.elems frame.allNodes).powerset
+    valuationsAsPsets.map ((@FiniteValuation.equivToFinSetRepresentation _ _ frame).symm.toEmbedding)
+
+  def satisfiesForAllValuations {frame : FiniteKripkeFrame n} (finVars : Type) [Fintype finVars] [DecidableEq finVars]
+                                (i : frame.vertices) (fml : ModalFormula finVars) : Bool :=
+    decide (∀finval ∈ frame.allValuations finVars, finval.valuation.decideSatisfaction i fml)
+
+  def countSatisfyingNodes (frame : FiniteKripkeFrame n)
+                           (fml : ModalFormula finVars) [Fintype finVars] [DecidableEq finVars] : ℕ :=
+    (frame.allNodes.filter (fun i => satisfiesForAllValuations finVars i fml)).card
+
+  lemma countSatisfyingNodes_leq_frameSize
+    (frame : FiniteKripkeFrame n) (fml : ModalFormula finVars)
+    [Fintype finVars] [DecidableEq finVars]: frame.countSatisfyingNodes fml ≤ n := by
+    simp only [FiniteKripkeFrame.countSatisfyingNodes]
+    simp only [← frame.allNodes_card_eq_frameSize]
+    apply Finset.card_filter_le
+end FiniteKripkeFrame
+
 inductive KripkeGameVars : Type
 | p
 | q
@@ -21,76 +109,12 @@ instance KripkeGameVars.fintype : Fintype KripkeGameVars :=
 
 def KripkeGameVars.all : Finset KripkeGameVars := Finset.univ
 
-inductive ModalFormula (vars : Type) : Type where
-| var : vars → ModalFormula vars
-| neg : ModalFormula vars → ModalFormula vars
-| and : ModalFormula vars → ModalFormula vars → ModalFormula vars
-| box : ModalFormula vars → ModalFormula vars
-
 namespace ModalFormula
   abbrev p := var KripkeGameVars.p
   abbrev q := var KripkeGameVars.q
   abbrev r := var KripkeGameVars.r
   abbrev s := var KripkeGameVars.s
-
-  variable {finVars : Type} [Fintype finVars] [DecidableEq finVars]
-
-  abbrev not := fun (φ: ModalFormula finVars) => neg φ
-  abbrev or := fun (φ1 φ2: ModalFormula finVars) => not (and (not φ1) (not φ2))
-  abbrev implies := fun (φ1 φ2: ModalFormula finVars) => or (not φ1) φ2
-  abbrev dia := fun (φ: ModalFormula finVars) => not (box (not φ))
 end ModalFormula
-
-/-- A Kripke frame of `frameSize` possible worlds is a directed graph with `frameSize` nodes.
-
-We think of the nodes in the graph as being numbered from `0` to `frameSize - 1`, inclusive,
-and we think the `j`-th node is accessible from the `i`-th node if and only if there is an edge from `i` to `j`.
-
-The graph, then, is represented by a function that takes two natural numbers `n` and `m` as input,
-and returns `true` if there is an edge from node `n` to node `m`, and `false` otherwise.
--/
-def KripkeFrame (frameSize : Nat) : Type := Fin frameSize → Fin frameSize → Bool
-namespace KripkeFrame
-  def Node (_ : KripkeFrame frameSize) := Fin frameSize
-  instance (frame : KripkeFrame n) : Fintype frame.Node := inferInstanceAs (Fintype (Fin n))
-  instance (frame : KripkeFrame n) : DecidableEq frame.Node := inferInstanceAs (DecidableEq (Fin n))
-
-  def allNodes (frame : KripkeFrame n) : Finset frame.Node := Finset.univ
-  lemma allNodes_card_eq_frameSize (frame : KripkeFrame n) : frame.allNodes.card = n :=
-    by apply Fintype.card_fin
-
-  def accessible (frame : KripkeFrame n) (i j : frame.Node) : Bool := frame i j
-  def accessibilityRelationCount (frame : KripkeFrame n) : ℕ :=
-    ((frame.allNodes.product (frame.allNodes)).filter (fun a => frame.accessible a.fst a.snd)).card
-
-  def Valuation (frame : KripkeFrame n) (vars : Type) : Type := vars → frame.Node → Bool
-
-  def Valuation.satisfiesAt {frame : KripkeFrame n} (i : frame.Node) (fml : ModalFormula vars) (val : frame.Valuation vars) : Bool :=
-  match fml with
-    | ModalFormula.var x => val x i
-    | ModalFormula.neg φ => !(val.satisfiesAt i φ)
-    | ModalFormula.and φ1 φ2 => val.satisfiesAt i φ1 && val.satisfiesAt i φ2
-    | ModalFormula.box φ => decide (∀j ∈ frame.allNodes, if frame.accessible i j then val.satisfiesAt j φ else true)
-
-  def Valuation.isoToFinSetEquiv {frame : KripkeFrame n}: (Finset (KripkeGameVars × frame.Node)) ≃ (frame.Valuation KripkeGameVars) :=
-    finsetProdEquivCurriedCharacteristic
-
-  def allValuations (frame : KripkeFrame n) : Finset (frame.Valuation KripkeGameVars) :=
-    let valuationsAsPsets := (Finset.product KripkeGameVars.all frame.allNodes).powerset
-    valuationsAsPsets.map ((@KripkeFrame.Valuation.isoToFinSetEquiv _ frame).toEmbedding)
-
-  def Node.satisfiesForAllValuations {frame : KripkeFrame n} (i : frame.Node) (fml : ModalFormula KripkeGameVars) : Bool :=
-    decide (∀val ∈ frame.allValuations, val.satisfiesAt i fml)
-
-  def countSatisfyingNodes (frame : KripkeFrame n) (fml : ModalFormula KripkeGameVars) : ℕ :=
-    (frame.allNodes.filter (fun i => i.satisfiesForAllValuations fml)).card
-
-  lemma countSatisfyingNodes_leq_frameSize
-    (frame : KripkeFrame n) (fml : ModalFormula KripkeGameVars) : frame.countSatisfyingNodes fml ≤ n := by
-    simp only [KripkeFrame.countSatisfyingNodes]
-    simp only [← frame.allNodes_card_eq_frameSize]
-    apply Finset.card_filter_le
-end KripkeFrame
 
 structure KripkeGameVisibleState where
   frameSize : ℕ
@@ -115,7 +139,7 @@ namespace KripkeGameVisibleState
   def withNewQueryAndAnswer (state : KripkeGameVisibleState) (query : ModalFormula KripkeGameVars) (answer : Fin (state.frameSize + 1)) : KripkeGameVisibleState :=
     { state with queriesAndAnswers := (query, answer) :: state.queriesAndAnswers }
 
-  def possibleFramesUptoIso (state : KripkeGameVisibleState) : Finset (KripkeFrame state.frameSize) :=
+  def possibleFramesUptoIso (state : KripkeGameVisibleState) : Finset (FiniteKripkeFrame state.frameSize) :=
     sorry
 
   def possibleFramesUptoIsoCard (state : KripkeGameVisibleState) : ℕ := state.possibleFramesUptoIso.card
